progress in assign

trans.v
@@ -102,6 +102,24 @@ Fixpoint move_gamma (G: source.context) (m: Syntax.term obj) (gamma: Syntax.term
      nil => gamma
    | A::xs => ppair (move_app A m (ppi1 gamma)) (move_gamma xs m (ppi2 gamma)) end.
 
+Definition eq_bbc: (term obj) := lam
+                         (
+                           (*f := 0*)
+                           lam ( (*f:= 1, n := 0*)
+                               lam ((*f := 2, n:= 1, m := 0*)
+                                   let f := (var 2) in
+                                   let n := (var 1) in
+                                   let m := (var 0) in
+                                                  bite (if_z n)
+                                                  (if_z m)
+                                                  (bite (if_z m)
+                                                     (bfalse)
+                                                    (app (app f (app (ppi2 n) triv)) (app (ppi2 m) triv)))
+                                                  ))).
+ Definition eq_b: (term obj) := app theta eq_bbc.
+
+Lemma eqb_typed {G}: tr G (oof eq_b (arrow nattp (arrow nattp booltp))).
+Admitted.
 
  Inductive trans: source.context -> source.term -> source.term -> (Syntax.term obj) -> Type :=
   t_bind: forall G E1 Et1 E2 Et2 A B, of_m G (bind_m E1 E2) (comp_m B) ->
@@ -185,60 +203,36 @@ that. you want to bind
                                  (ppair l (ppair triv (lam triv)) (*ref A @ new world*)
                                  ) 
                           )
-                   ))))))).
-  | t_ref: forall G E Et A, 
-         of_m G (ref_m E) (comp_m (reftp_m A)) -> trans G E A Et ->
-         trans G (ref_m E) (comp_m (reftp_m A)) (lam (lam (lam (lam ( lam ( (*l1, g, l, m, s*)
-         let l := var 2 in                                                        
-         let m1 := make_subseq in (*u <= u1)*)
-         let p1 := (ppair m1
-                         (lam (lam ( lam ( (*making a value of type store U1, lambdas go l2, m2, i*)
-                                         let l1 := var 7 in
-                                         let g := var 6 in
-                                         let l := var 5 in
-                                         let s := var 3 in
-                                         let l2 := var 2 in
-                                         let i := var 0 in
-                                         let x := app (app (shift 8 Et) l1) g in
-                                         let m12 := make_subseq in (*m2 o m1 : U <= U2*)
-                                         let m02 := make_subseq in (*m12 o m : W <= U2*)
-                                         bite (app (app lt_b i) l)
-                                              (app (app (app s l2) m12) i) (*move value in s:store(U) to U2*)
-                                              (next (move_app A m02 x)) (*move x to be : |> A @ U2*)
-                                               ))
-                         ))
-         ) in
-             ret_a (ppair (nsucc l) (*length of new world*)
-                          (ppair p1 (*new word is accessible from current world, *)
-                                 (ppair l (ppair triv (lam triv)) (*ref A @ new world*)
-                                 ) 
-                          )
-                                                )))))))
+                   )))))))
   | t_assign: forall G R Rt E Et A,
       of_m G R (reftp_m A) ->
       of_m G E A ->
       trans G R A Rt ->
       trans G E A Et ->
-      trans G (asgn_m R E)
+      trans G (asgn_m R E) (comp_m unittp_m)
             (lam (lam (lam (lam ( lam ( (*l = 4, g = 3, l1 = 2, m = 1, s1 = 0*)
-                                      let m = var 1 in
-                                      let l1 = var 2 in
-                                      let s1 = var 0 in 
-                                      let ref =move_app (reftp_m A) m (app (app Rt l) g) in
-                                      let i = ppi1 ref in
-                                      let p = ppi2 ref in
-                                      let store_u1  = lam (lam (lam (*l2 = 2, m1 = 1,j = 0*)
+                                      let l := var 4 in
+                                      let m := var 1 in
+                                      let l1 := var 2 in
+                                      let g := var 3 in
+                                      let s1 := var 0 in 
+                                      let ref := move_app (reftp_m A) m (app (app (shift 5 Rt) l) g) in
+                                      let i := ppi1 ref in
+                                      let p := ppi2 ref in
+                                      let store_u1  := lam (lam (lam (*l2 = 2, m1 = 1,j = 0*)
                                                                   (
-                                                                    let j = (var 0) in
-                                                                    let l2 = var 2 in
-                                                                    let i = shift 3 i in
+                                                                    let j := (var 0) in
+                                                                    let l2 := var 2 in
+                                                                    let i := shift 3 i in
+                                                                    let l := shift 3 l in
                                                                     bite
-                                                                      (eq_b j i)
-                                                                      (next (move_app A (make_subseq) (app (app Et) g)))
+                                                                      (app (app eq_b j) i)
+                                                                      (next (move_app A (make_subseq)
+                                                                                      (app (app (shift 8 Et) l) g)))
                                                                       (app (app (app (shift 3 s1) l2) make_subseq) j)
                                                                  ))) in
                                       ret_a (ppair l1
                                                    (ppair
                                                       (ppair make_subseq store_u1)
                                                       triv))
-                                            ))))))
+                                            )))))).
